Mt/samples/sample_mutex.lean
@@ -1,0 +1,120 @@
+import Mt.Reservation
+import Mt.Task
+import Mt.System
+
+structure State where
+  x : Nat
+  y : Nat
+
+def State.valid : State -> Prop
+| ⟨x, y⟩ => x = y
+
+abbrev Reservation :=Mt.Lock State
+
+inductive validate : Reservation -> State -> Prop where
+| unlocked {s : State} : s.valid → validate Mt.Lock.Unlocked s
+| locked (s : State) : validate (Mt.Lock.Locked s) s
+
+def spec : Mt.Spec :={
+  State
+  Reservation
+  validate
+}
+
+open Mt
+open Mt.TaskM
+
+/-- read-modify operation assuming the mutex is owned -/
+abbrev rm_locked (f : State -> State) : TaskM spec Unit :=
+  atomic_read_modify λ _ s => match f s with
+    | s' => ⟨Lock.Locked s', s'⟩ 
+
+def thread1 : TaskM spec Unit :=do
+  -- lock mutex
+  atomic_blocking_rmr (λ r => r.is_unlocked) λ _ s => ⟨⟨⟩, Mt.Lock.Locked s, s⟩
+  
+  -- two atomic modifications, one after the other
+  rm_locked λ s => {s with x :=s.x + 1}
+  rm_locked λ s => {s with y :=s.y + 1}
+  
+  -- release mutex
+  atomic_read_modify λ _ s => ⟨Mt.Lock.Unlocked, s⟩
+
+def thread2 : TaskM spec Unit :=do
+  -- lock mutex
+  atomic_blocking_rmr (λ r => r.is_unlocked) λ _ s => ⟨⟨⟩, Mt.Lock.Locked s, s⟩
+  
+  -- two atomic reads, one after the other
+  let px <- atomic_read λ r ⟨x, _⟩ => ⟨x, r⟩
+  let py <- atomic_read λ r ⟨_, y⟩ => ⟨y, r⟩
+
+  atomic_assert λ _ => px = py
+  
+  -- release mutex
+  atomic_read_modify λ _ s => ⟨Mt.Lock.Unlocked, s⟩
+
+theorem validate.elim_unlocked {r s} :
+  validate r s → r.is_unlocked → s.valid :=by
+  intro initial_valid unlocked
+  cases initial_valid
+  . assumption
+  . contradiction
+
+theorem validate.elim_locked {env_r : Reservation} {s s'} :
+  validate (env_r + Lock.Locked s) s' →
+  env_r = Lock.Unlocked ∧ s = s' :=by
+  intro initial_valid
+  cases env_r <;> cases initial_valid
+  exact ⟨rfl, rfl⟩
+
+theorem thread1_valid : thread1.valid' Mt.Lock.Unlocked :=by
+  rw [valid']
+  apply valid_bind (spec :=spec) λ ⟨⟩ r => r.is_locked_and_valid State.valid
+  . -- verify mutex lock
+    apply valid_blocking_rmr
+    simp only [spec, Lock.add_unlocked]
+    intro env_r s is_unlocked initial_valid
+    have :=Lock.eq_of_is_unlocked is_unlocked
+    simp only [spec, this, Lock.unlocked_add, Lock.is_locked_and_valid]
+    exact ⟨validate.locked .., initial_valid.elim_unlocked is_unlocked⟩
+  
+  intro r ⟨⟩ is_locked_and_valid
+  cases r <;> try contradiction
+  rename_i s0
+  let ⟨x0, y0⟩ :=s0 ; clear s0
+  cases is_locked_and_valid
+  apply valid_bind (spec :=spec) λ ⟨⟩ r' => r' = Lock.Locked ⟨x0 + 1, x0⟩
+  . -- validate ++x
+    apply valid_rm
+    simp only [spec]
+    intro env_r ⟨x, y⟩ ⟨⟩ initial_valid
+    simp only [initial_valid.elim_locked, Lock.unlocked_add]
+    injection initial_valid.elim_locked.right
+    rename_i x0_def y0_def
+    simp only [<- x0_def, <- y0_def]
+    exact ⟨validate.locked _, ⟨⟩⟩
+  
+  intro r ⟨⟩ r_def
+  rw [r_def] ; clear r_def r
+  apply valid_bind (spec :=spec) λ ⟨⟩ r' => r' = Lock.Locked ⟨x0 + 1, x0 + 1⟩
+  . -- validate ++y
+    apply valid_rm
+    simp only [spec]
+    intro env_r ⟨x, y⟩ ⟨⟩ initial_valid
+    simp only [initial_valid.elim_locked, Lock.unlocked_add]
+    injection initial_valid.elim_locked.right
+    rename_i x0_def y0_def
+    simp only [<- x0_def, <- y0_def]
+    exact ⟨validate.locked _, ⟨⟩⟩
+
+  intro r ⟨⟩ r_def
+  rw [r_def]; clear r_def r
+  . -- validate mutex release
+    apply valid_rm
+    simp only [spec, Lock.add_unlocked]
+    intro env_r ⟨x, y⟩ ⟨⟩ initial_valid
+    injection initial_valid.elim_locked.right
+    rename_i x_def y_def
+    simp only [initial_valid.elim_locked]
+    rw [x_def.symm, y_def.symm] ; clear x_def y_def
+    exact ⟨validate.unlocked rfl, rfl⟩
